type checking well formed.

src/SmallCoreTypeAlg.v
@@ -27,3 +27,218 @@ Theorem has_type_dec:
 
 Abort.
 
+Fixpoint check_type (ctx : Context (type := {x : ty | wf_ty x})) (t : tm) : option ty.
+    refine
+    (match t with
+        | tvar i => _
+        | tnone => Some TNone
+        | tfun i T h body => match (check_type (update i (exist wf_ty T h) ctx) body) with
+                                | None => None 
+                                | Some o => _
+                             end
+        | tapp f x => _
+        | tlet i T h bind body => _
+        | tfixApp i T h self => _
+        | tleft lt RT h => _
+        | tright LT h rt => _
+
+        | tcase crit lf rf => _
+        | trcons i head tail => _
+        | text T t h => Some (extty_to_ty T)
+        | tfield T h0 h1 i => _
+    end
+    ).
+
+
+    Ltac NotNoneInCtx :=
+        match goal with
+        | h : _ = None |- _ => exact None 
+        | h : None = _ |- _ => exact None 
+        | |- _ => idtac
+        end.
+    Ltac AssertORFU Tx :=
+        destruct (orfu_dec Tx);
+        match goal with
+        | h : ~orfu Tx |- _ => exact None
+        | |- _ => idtac
+        end.
+
+    (* case tvar *)
+    destruct (byContext ctx i) eqn:h0; NotNoneInCtx.
+    destruct s. 
+    AssertORFU x.
+    exact (Some x).
+
+    (* case tfun *)
+    AssertORFU T. exact (Some (TFun T o)).
+
+
+    (* case tapp *)
+    destruct (check_type ctx f) eqn:h0; NotNoneInCtx.
+    destruct t0 eqn: h1;
+    match goal with
+    | h : t0 = TFun ?I ?O |- _ =>
+        destruct (check_type ctx x) eqn:h2;
+        NotNoneInCtx
+    | |- _ => exact None
+    end; NotNoneInCtx.
+    destruct (subty_dec t1 t1_1).
+    exact (Some t1_2).
+    (* when ~ x <: I*)
+    exact None.
+
+    (* case tlet *)
+    destruct (check_type ctx bind) eqn:h0;
+    NotNoneInCtx.
+    destruct (eq_ty_dec T t0).
+    destruct (check_type (update i (exist wf_ty T h) ctx) body) eqn:h1;
+    NotNoneInCtx.
+    exact (Some t1). exact None.
+
+    (* case tfixApp *)
+    destruct (check_type (update i (exist wf_ty T h) ctx) self) eqn: h0; NotNoneInCtx.
+    destruct (subty_dec t0 T). exact (Some T). exact None. 
+
+    (* case tleft *)
+    destruct (check_type ctx lt) eqn: h0; NotNoneInCtx.
+    AssertORFU RT.
+    exact (Some (TSum t0 RT)).
+
+    (* case tright *)
+    destruct (check_type ctx rt) eqn: h0; NotNoneInCtx.
+    AssertORFU LT.
+    exact (Some (TSum LT t0)).
+
+    (* case tcase *)
+    destruct (check_type ctx crit) eqn:h0;
+    destruct (check_type ctx lf) eqn:h1;
+    destruct (check_type ctx rf) eqn:h2;
+    NotNoneInCtx.
+        (* crit must be sum*)
+        destruct t0 eqn:h3;
+        match goal with
+        | h : t0 = TSum _ _ |- _ => idtac
+        | |- _ => exact None
+        end.
+        (* lf, rf must be a function*)
+        destruct t1 eqn:h4;
+        match goal with
+        | h : t1 = TFun _ _ |- _ => idtac
+        | |- _ => exact None
+        end;
+        destruct t2 eqn:h5;
+        match goal with
+        | h : t2 = TFun _ _ |- _ => idtac
+        | |- _ => exact None
+        end.
+        destruct (subty_dec t3_1 t3_3);
+        destruct (subty_dec t3_2 t3_5);
+        destruct (eq_ty_dec t3_4 t3_6);
+        subst; 
+        match goal with
+        | h0 : check_type ctx crit = Some (TSum ?li ?ri),
+          h1 : check_type ctx lf = Some (TFun ?li' ?o),
+          h2 : check_type ctx rf = Some (TFun ?ri' ?o),
+          h3 : subty ?li ?li' ,
+          h4 : subty ?ri ?ri'
+          |- _ => exact o
+        | |- _ => exact None
+        end.
+    
+        (* case trcons *)
+        destruct (check_type ctx head) eqn: h0; 
+        destruct (check_type ctx tail) eqn: h1;
+        NotNoneInCtx.
+        destruct (only_rcd_dec t1).
+        destruct (rcd_field_ty' t1 i) eqn: h2.
+        exact None.
+        AssertORFU t1.
+        exact (Some (TRcons i t0 t1)).
+        exact None.
+
+        (* case tfield *)
+        destruct (rcd_field_ty T h0 h1 i) eqn: h2;
+        NotNoneInCtx.
+        AssertORFU T. AssertORFU t0.
+        exact (Some (TFun T t0)).
+
+Defined.
+
+
+Theorem typing_alg_well_formed:
+    forall ctx t T,
+        check_type ctx t = Some  T ->
+        wf_ty T.
+
+Proof with eauto; try discriminate.
+    intros ctx t. glize ctx 0.
+    induction t; intros; cbn in *; subst; eauto; try discriminate;
+    repeat (
+        match goal with
+        | h : (match ?x with _ => _ end) _ = _ |- _ =>
+            let h := fresh c in
+            destruct x eqn:h
+        | h : (match ?x with _ => _ end) _ _ = _ |- _ =>
+            let h := fresh c in
+            destruct x eqn:h
+        | h : (match ?x with _ => _ end) = _ |- _ =>
+            let h := fresh c in
+            destruct x eqn:h
+        | h : (if ?x then _ else _) = _ |- _ =>
+            let h := fresh c in
+            destruct x
+        | h : Some _ = Some _ |- _ => inversion h; subst;eauto; try discriminate; clear h
+        end;eauto; try discriminate
+    );subst ...
+
+    (* case tapp *)
+    forwards*: IHt1...
+    forwards*: IHt2...
+    inversion H; eauto.
+
+    (* case text *)
+    eapply Extty_well_formed.
+
+
+    (* case tfield *)
+    eapply wfFun; eauto.
+    unfold rcd_field_ty in *.
+    eapply rcd_field_ty'_wf_is_wf; eauto.
+Qed.
+
+
+
+
+
+
+   
+
+
+Theorem typing_alg_leg:
+    forall ctx t T,
+        check_type ctx t = Some T ->
+        has_type ctx t T.
+
+    intros ctx t. glize ctx 0.
+    induction t; intros; subst; cbn in *; eauto; try discriminate.
+    
+    (* TNone *)
+    destruct (byContext ctx i) eqn:h0.
+    destruct s; eauto.
+    destruct (orfu_dec x); subst; eauto; try discriminate.
+    inversion H; subst; eauto.
+    try discriminate.
+    inversion H; subst; eauto.
+    
+
+    (* TFun *)
+    destruct (check_type (update i (exist wf_ty T w) ctx) t) eqn:h0.
+    destruct (orfu_dec T); subst; eauto; try discriminate.
+    inversion H; subst; eauto.
+    try discriminate.
+
+    (* case tapp *)
+    destruct (check_type ctx t1) eqn:h0.
+    destruct t. destruct (check_type ctx t2) eqn:h1.
+    destruct (subty_dec t t3); eauto. inversion H; subst; eauto.
+    eapply ht_app; eauto.
